ratchet/Denote/Sem/Transport.lean
@@ -224,7 +224,9 @@ theorem Framed.of_ext {m m' : Machine} (he : Ext m m') : Framed m m' :=
     fun v n h => by
       simpa only [denM] using
         (denM_ext (τ := .cls n) (v := v) he (by simpa only [denM] using h)),
-    fun _ _ _ h => denM_ext he h, .of_eq he.stack he.frames⟩
+    fun _ _ _ h => denM_ext he h, .of_eq he.stack he.frames,
+    .of_unchanged he.size (fun o ho => by funext x; simp only [ivarOf, he.get o ho])
+      (fun _ _ _ h => denM_ext he h)⟩
 
 theorem Framed_withCtl (m : Machine) (c : Ctl) : Framed m (Interp.withCtl m c) :=
   Framed.of_heap_stack rfl rfl (.of_eq rfl rfl)
